

DIFFERENTIATION

LIST OF DEVRIVATIVES

$$1] \frac{d}{dx}(x^n) = nx^{n-1}, 2] \frac{d}{dx}(x) = 1, 3] \frac{d}{dx}(x^2) = 2x^{2-1} = 2x, 4] \frac{d}{dx}(x^3) = 3x^{3-1} = 3x^2$$

$$5] \frac{d}{dx}(x^4) = 4x^{4-1} \quad 6] \frac{d}{dx}\left(\frac{1}{x}\right) = -\frac{1}{x^2}, 7] \frac{d}{dx}(\sqrt{x}) = \frac{1}{2\sqrt{x}}, 8] \frac{d}{dx}(e^x) = e^x$$

$$9] \frac{d}{dx}(\log x) = \frac{1}{x} \quad 10] \frac{d}{dx}(\sin x) = \cos x, 11] \frac{d}{dx}(\cos x) = -\sin x,$$

$$12] \frac{d}{dx}(\tan x) = \sec^2 x, 13] \frac{d}{dx}(\cot x) = -\operatorname{cosec}^2 x, 14] \frac{d}{dx}(\sec x) = \sec x \tan x$$

$$15] \frac{d}{dx}(\operatorname{cosec} x) = -\operatorname{cosec} x \cot x, 16] \frac{d}{dx}(\sin^{-1} x) = \frac{1}{\sqrt{1-x^2}},$$

$$17] \frac{d}{dx}(\cos^{-1} x) = -\frac{1}{\sqrt{1-x^2}}, 18] \frac{d}{dx}(\tan^{-1} x) = \frac{1}{1+x^2} \quad 19] \frac{d}{dx}(\text{any number}) = 0$$

$$20] \frac{d}{dx}(ax) = a \frac{d}{dx}(x)$$

$$1) \text{ Evaluate } \lim_{x \rightarrow 0} \frac{2x-3}{3x+5} = \frac{2 \times 0 - 3}{3 \times 0 + 5} = \frac{0-3}{0+5} = -\frac{3}{5}$$

2) State product rule of differentiation

$$\frac{d}{dx}(uv) = u \frac{dv}{dx} + v \frac{du}{dx} = \text{First function} \times \frac{d}{dx}(\text{second}) + \text{second} \times \frac{d}{dx}(\text{first})$$

3) Differentiate $y = \log x$ w.r to x

to find derivatives of terms in y , multiply with $\frac{dy}{dx}$

ANS: $x^2 + y^2 = 25$, Taking derivatives, $\frac{d}{dx}(x^2 + y^2) = \frac{d}{dx}(25)$

$$2x + 2y \times \frac{dy}{dx} = 0, \quad 2y \times \frac{dy}{dx} = -2x, \quad \frac{dy}{dx} = \frac{-2x}{2y} = -\frac{x}{y}$$

5) If $y = \sin x$, find $\frac{d^2y}{dx^2}$

$$\frac{dy}{dx} = \frac{d}{dx}(\sin x) = \cos x$$

$$\frac{d^2y}{dx^2} = \text{derivative of } \frac{dy}{dx} = \frac{d}{dx}(\cos x) = -\sin x$$

6) Evaluate $\lim_{\theta \rightarrow 0} \frac{\sin 3\theta}{3\theta}$

$$\lim_{\theta \rightarrow 0} \frac{\sin a\theta}{a\theta} = 1$$

$$\lim_{\theta \rightarrow 0} \frac{\sin 3\theta}{3\theta} = 1, a = 3$$

7) Differentiate $e^x \sin x$ with respect to x

$$\frac{d}{dx}(e^x) = e^x, \quad \frac{d}{dx}(\sin x) = \cos x$$

$$\frac{d}{dx}(e^x \sin x) = \text{First function} \times \frac{d}{dx}(\text{second}) + \text{second} \times \frac{d}{dx}(\text{first})$$

$$= e^x \times \frac{d}{dx}(\sin x) + \sin x \times \frac{d}{dx}(e^x) = e^x \times \cos x + \sin x \times e^x$$

8) Differentiate $\frac{\sin x}{1 + \cos x}$ with respect to x

Quotient Rule

$$\frac{\text{Denominator} \times \frac{d}{dx}(\text{numerator}) - \text{numerator} \times \frac{d}{dx}(\text{denominator})}{\text{denominator}^2}$$

$$y = \frac{\sin x}{1 + \cos x}, \quad \text{Numerator} = \sin x, \quad \text{Denominator} = 1 + \cos x$$

$$\frac{dy}{dx} = \frac{(1 + \cos x) \times \frac{d}{dx}(\sin x) - \sin x \times \frac{d}{dx}(1 + \cos x)}{(1 + \cos x)^2}$$

$$= \frac{(1 + \cos x) \times \cos x - \sin x \times (0 + -\sin x)}{(1 + \cos x)^2} = \frac{(1 + \cos x) \times \cos x - \sin x \times (-\sin x)}{(1 + \cos x)^2}$$

$$= \frac{(1 + \cos x) \times \cos x + \sin^2 x}{(1 + \cos x)^2}$$



9) $x = a \sec \theta, y = b \tan \theta$, find $\frac{dy}{dx}$

$$\frac{d}{dx}(\tan x) = \sec^2 x, \frac{d}{d\theta}(\tan \theta) = \sec^2 \theta$$

$$\frac{dy}{dx} = \frac{\frac{dy}{d\theta}}{\frac{dx}{d\theta}}$$

$$\frac{dy}{d\theta}, y = b \tan \theta, \frac{dy}{d\theta} = b \sec^2 \theta$$

derivative of, $\sec x = \sec x \tan x$, derivative of a $\sec x = a \times \sec x \tan x$

$$\frac{dx}{d\theta}, x = a \sec \theta, \frac{dx}{d\theta} = a \sec \theta \tan \theta,$$

$$\frac{dy}{dx} = \frac{\frac{dy}{d\theta}}{\frac{dx}{d\theta}}, \frac{dy}{dx} = \frac{b \sec^2 \theta}{a \sec \theta \tan \theta} = \frac{b \sec \theta}{a \tan \theta} = \frac{b}{a} \times \frac{\frac{1}{\cos \theta}}{\frac{\sin \theta}{\cos \theta}}$$

$$= \frac{b}{a} \times \frac{1}{\sin \theta} = \frac{b}{a} \operatorname{cosec} \theta$$

$$\frac{1}{\cos \theta} = \sec \theta, \frac{\sin \theta}{\cos \theta} = \tan \theta, \frac{1}{\sin \theta} = \operatorname{cosec} \theta$$

10) Find the second derivative of $x \log x$

$x \log x$ is a product, First function x , second function $\log x$

$$\text{First derivative} = \frac{dy}{dx} = \frac{d}{dx}(x \log x)$$

$$\frac{d}{dx}(x \log x) = \text{First function} \times \frac{d}{dx}(\text{second}) + \text{second} \times \frac{d}{dx}(\text{first})$$

$$= x \times \frac{d}{dx}(\log x) + \log x \times \frac{d}{dx}(x) = x \times \frac{1}{x} + \log x \times 1 = 1 + \log x,$$

$$\bullet x \times \frac{1}{x} = 1$$

11) $\lim_{x \rightarrow a} \frac{x^n - a^n}{x - a} = na^{n-1}$, Evaluate $\lim_{x \rightarrow 3} \frac{x^4 - 81}{x^2 - 9}$, $81 = 3 \times 3 \times 3 \times 3 = 3^4$, $9 = 3^2$

$$\lim_{x \rightarrow 3} \frac{x^4 - 3^4}{x^2 - 3^2}, \text{divide numerator and denominator with } x - 3, \lim_{x \rightarrow 3} \frac{\frac{x^4 - 3^4}{x - 3}}{\frac{x^2 - 3^2}{x - 3}}$$

$$\lim_{x \rightarrow 3} \frac{\frac{x^4 - 3^4}{x - 3}}{\frac{x^2 - 3^2}{x - 3}} = \frac{4 \times 3^{4-1}}{2 \times 3^{2-1}} = \frac{4 \times 3^3}{2 \times 3^1} = \frac{4 \times 3 \times 3 \times 3}{2 \times 3} = 18$$

12) Differentiate with respect to $x, y = x^2 \sec x$,

$$\frac{d}{dx}(x^2) = 2x, \frac{d}{dx}(\sec x) = \sec x \tan x$$

$y = x^2 \sec x$, use product rule

$$\frac{d}{dx}(x^2 \sec x) = \text{First function} \times \frac{d}{dx}(\text{second}) + \text{second} \times \frac{d}{dx}(\text{first})$$

$$= x^2 \times \frac{d}{dx}(\sec x) + \sec x \times \frac{d}{dx}(x^2) = x^2 \times \sec x \tan x + \sec x \times 2x$$

13) Differentiate with respect to x , $y = \frac{1-x^2}{1+x^2}$, use quotient rule

$$\frac{d}{dx}(x^2) = 2x, \frac{d}{dx}(1) = 0$$

$$\frac{d}{dx}\left(\frac{1-x^2}{1+x^2}\right) = \frac{\text{Denominator} \times \frac{d}{dx}(\text{numerator}) - \text{numerator} \times \frac{d}{dx}(\text{denominator})}{\text{denominator}^2}$$

$$\text{Numerator} = 1 - x^2, \text{Denominator} = 1 + x^2$$

$$\frac{dy}{dx} = \frac{d}{dx}\left(\frac{1-x^2}{1+x^2}\right) = \frac{(1+x^2) \times \frac{d}{dx}(1-x^2) - (1-x^2) \times \frac{d}{dx}(1+x^2)}{(1+x^2)^2}$$

$$= \frac{(1+x^2) \times (0-2x) - (1-x^2) \times (0+2x)}{(1+x^2)^2} = \frac{(1+x^2) \times (-2x) - (1-x^2) \times (2x)}{(1+x^2)^2}$$

14) Find the derivative of $\tan x$ using quotient rule

$$\tan x = \frac{\sin x}{\cos x}, \frac{d}{dx}(\sin x) = \cos x, \frac{d}{dx}(\cos x) = -\sin x, \cos^2 x + \sin^2 x = 1$$

$$\text{Numerator} = \sin x, \text{Denominator} = \cos x$$

$$\frac{d}{dx}(\tan x) = \frac{d}{dx}\left(\frac{\sin x}{\cos x}\right) = \frac{\text{Denominator} \times \frac{d}{dx}(\text{numerator}) - \text{numerator} \times \frac{d}{dx}(\text{denominator})}{\text{denominator}^2}$$

$$= \frac{(\cos x) \times \frac{d}{dx}(\sin x) - (\sin x) \times \frac{d}{dx}(\cos x)}{(\cos x)^2} = \frac{(\cos x) \times (\cos x) - (\sin x) \times (-\sin x)}{(\cos x)^2}, (-) \times (-) = +$$

$$= \frac{\cos^2 x + \sin^2 x}{(\cos x)^2} = \frac{1}{\cos^2 x} = \sec^2 x, \frac{1}{\cos x} = \sec x, (\cos x)^2 = \cos^2 x$$

15) Find the derivative of $\cot x$ using quotient rule

$$\cot x = \frac{\cos x}{\sin x}, \frac{d}{dx}(\sin x) = \cos x, \frac{d}{dx}(\cos x) = -\sin x, \sin^2 x + \cos^2 x = 1$$

$$\frac{d}{dx}(\cot x) = \frac{d}{dx}\left(\frac{\cos x}{\sin x}\right) = \frac{\text{Denominator} \times \frac{d}{dx}(\text{numerator}) - \text{numerator} \times \frac{d}{dx}(\text{denominator})}{\text{denominator}^2}$$

$$\frac{(\sin x) \times \frac{d}{dx}(\cos x) - (\cos x) \times \frac{d}{dx}(\sin x)}{(\sin x)^2} = \frac{(\sin x) \times (-\sin x) - (\cos x) \times (\cos x)}{(\sin x)^2}, (+) \times (-) = -$$

$$= \frac{-\sin^2 x - \cos^2 x}{(\sin x)^2} = \frac{-(\sin^2 x + \cos^2 x)}{(\sin x)^2} = \frac{-1}{\sin^2 x} = -\operatorname{cosec}^2 x$$

$$16) x = a(\theta - \sin\theta), y = a(1 - \cos\theta), \text{ find } \frac{dy}{dx}, \frac{dy}{dx} = \frac{\frac{dy}{d\theta}}{\frac{dx}{d\theta}}$$

$$\frac{d}{dx}(\sin x) = \cos x, \frac{d}{d\theta}(\sin\theta) = \cos\theta, \frac{d}{d\theta}(\cos\theta) = -\sin\theta, \frac{d}{dx}(1) = 0, \frac{d}{d\theta}(1) = 0$$

$$y = a(1 - \cos\theta), \frac{dy}{d\theta} = a(0 - -\sin\theta), a(- -\sin\theta) = a\sin\theta, - - = +$$

$$\frac{d}{dx}(x) = 1, \frac{d}{d\theta}(\theta) = 1, x = a(\theta - \sin\theta), \frac{dx}{d\theta} = a(1 - \cos\theta)$$

$$\frac{dy}{dx} = \frac{\frac{dy}{d\theta}}{\frac{dx}{d\theta}} = \frac{a\sin\theta}{a(1 - \cos\theta)}$$

$$17) x = at^2, y = 2at, \text{ find } \frac{dy}{dx}, \frac{dy}{dx} = \frac{\frac{dy}{dt}}{\frac{dx}{dt}}, \frac{d}{dx}(x) = 1, \frac{d}{dt}(t) = 1,$$

$$\frac{d}{dx}(x^2) = 2x, \frac{d}{dx}(t^2) = 2t$$

$$y = 2at, \frac{dy}{dt} = \frac{d}{dt}(2at) = 2a \times \frac{d}{dt}(t) = 2a \times 1 = 2a$$

$$x = at^2, \frac{dx}{dt} = \frac{d}{dt}(at^2) = a \times 2t = 2at$$

$$\frac{dy}{dx} = \frac{\frac{dy}{dt}}{\frac{dx}{dt}} = \frac{2a}{2at} = \frac{1}{t}$$

$$18) \text{ If } y = x \sin x, \text{ prove that } \frac{d^2y}{dx^2} + y = 2 \cos x$$

$y = x \sin x$, product, use product rule

$$\frac{d}{dx}(x \sin x) = \text{First function} \times \frac{d}{dx}(\text{second}) + \text{second} \times \frac{d}{dx}(\text{first})$$

$$= x \times \frac{d}{dx}(\sin x) + \sin x \times \frac{d}{dx}(x) = x \times (\cos x) + \sin x \times 1 = x(\cos x) + \sin x$$

$$\frac{d^2y}{dx^2} = \frac{d}{dx}[x(\cos x) + \sin x] = \frac{d}{dx}[x(\cos x)] + \frac{d}{dx}(\sin x) =$$

$$\text{First function} \times \frac{d}{dx}(\text{second}) + \text{second} \times \frac{d}{dx}(\text{first}) + \frac{d}{dx}(\sin x)$$

$$= x \times \frac{d}{dx}(\cos x) + \cos x \times \frac{d}{dx}(x) + \cos x = x \times -\sin x + \cos x \times 1 + \cos x$$

$$= -x\sin x + \cos x + \cos x = -x\sin x + 2\cos x, y = x \sin x$$

$$\frac{d^2y}{dx^2} + y = -x\sin x + 2\cos x + x\sin x = 2 \cos x$$

$$19) y = \log(\sec x + \tan x), \text{ find } \frac{dy}{dx}, \frac{d}{dx}(\log x) = \frac{1}{x}$$

$$\frac{d}{dx}(\sec x) = \sec x \tan x, \frac{d}{dx}(\tan x) = \sec^2 x$$



18) If $y = x \sin x$, prove that $\frac{d^2y}{dx^2} + y = 2 \cos x$

$y = x \sin x$, product, use product rule

$$\frac{d}{dx}(x \sin x) = \text{First function} \times \frac{d}{dx}(\text{second}) + \text{second} \times \frac{d}{dx}(\text{first})$$

$$= x \times \frac{d}{dx}(\sin x) + \sin x \times \frac{d}{dx}(x) = x \times (\cos x) + \sin x \times 1 = x(\cos x) + \sin x$$

$$\frac{d^2y}{dx^2} = \frac{d}{dx}[x(\cos x) + \sin x] = \frac{d}{dx}[x(\cos x)] + \frac{d}{dx}(\sin x) =$$

$$\text{First function} \times \frac{d}{dx}(\text{second}) + \text{second} \times \frac{d}{dx}(\text{first}) + \frac{d}{dx}(\sin x)$$

$$= x \times \frac{d}{dx}(\cos x) + \cos x \times \frac{d}{dx}(x) + \cos x = x \times -\sin x + \cos x \times 1 + \cos x$$

$$= -x \sin x + \cos x + \cos x = -x \sin x + 2 \cos x, y = x \sin x$$

$$\frac{d^2y}{dx^2} + y = -x \sin x + 2 \cos x + x \sin x = 2 \cos x$$

19) $y = \log(\sec x + \tan x)$, find $\frac{dy}{dx}$, $\frac{d}{dx}(\log x) = \frac{1}{x}$

$$\frac{d}{dx}(\sec x) = \sec x \tan x, \frac{d}{dx}(\tan x) = \sec^2 x$$

$$\begin{aligned} \text{Ans: } y = \log(\sec x + \tan x), \frac{dy}{dx} &= \frac{1}{(\sec x + \tan x)} \times \frac{d}{dx}(\sec x + \tan x) \\ &= \frac{1}{(\sec x + \tan x)} (\sec x \tan x + \sec^2 x) \end{aligned}$$

20) $y = \sin 2x$, find $\frac{dy}{dx}$, $\frac{d}{dx}(\sin x) = \cos x$, $\frac{d}{dx}(2x) = 2$,

$$\frac{d}{dx}(\sin 2x) = \cos 2x \times 2$$

21) $y = e^{\log x}$, find $\frac{dy}{dx}$, $\frac{d}{dx}(e^x) = e^x$, $\frac{d}{dx}(\log x) = \frac{1}{x}$,

$$\frac{d}{dx}(e^{\log x}) = (e^{\log x}) \times \frac{d}{dx}(\log x) = (e^{\log x}) \times \frac{1}{x}$$

22) $y = \frac{\sin 2x}{1 + \cos 2x}$, find $\frac{dy}{dx}$ (use quotient rule), $\frac{d}{dx}(\sin 2x) = \cos 2x \times 2$

$$\frac{d}{dx}(\cos 2x) = -\sin 2x \times 2, \frac{d}{dx}(1) = 0$$

$$\frac{d}{dx}\left(\frac{\sin 2x}{1 + \cos 2x}\right) = \frac{\text{Denominator} \times \frac{d}{dx}(\text{numerator}) - \text{numerator} \times \frac{d}{dx}(\text{denominator})}{\text{denominator}^2}$$

$$= \frac{(1 + \cos 2x) \times \frac{d}{dx}(\sin 2x) - (\sin 2x) \times \frac{d}{dx}(1 + \cos 2x)}{(1 + \cos 2x)^2} =$$

$$\frac{(1 + \cos 2x) \times \cos 2x \times 2 - (\sin 2x) \times (0 - \sin 2x \times 2)}{(1 + \cos 2x)^2}$$